\subsubsection{Structure of Full Hessian of the First Layer}
\label{sec:proof-full-hessian}
We first restate \theoremref{thm:main-full} here:

\noindent\textbf{\theoremref{thm:main-full}:}\emph{
Let $V_1$ and $V_2$ be the top $c-1$ eigenspaces of $\mH$ and $\hat\mH$ respectively, for all $\eps>0$, 
\begin{equation}
    \lim_{n\to\infty}\mathop{\Pr}_{\mW^{(1)}\sim\gN(0,\frac{1}{d}\mI_{nd}), \mW^{(2)}\sim\gN(0,\frac{1}{n}\mI_{cn})}\left[\Overlap\left(V_1,V_2\right)>1-\eps\right] = 1.
\end{equation}
Moreover, \begin{equation}
    \lim_{n\to\infty}\mathop{\Pr}_{\mW^{(1)}\sim\gN(0,\frac{1}{d}\mI_{nd}), \mW^{(2)}\sim\gN(0,\frac{1}{n}\mI_{cn})}\left[\left(\left.\frac{\lambda_c(\mH)}{\lambda_{c-1}(\mH)}\right|_{\mW^{(1)}, \mW^{(2)}}\right) < \eps\right] = 1.
\end{equation}
}

Before proceeding to the main theorem, we will first look into the eigenspectrum of the scaled auto-correlation matrix $\trmX\triangleq \frac1d\ex{\rvx\rvx^\T}$ and the top eigenspace of $\hat\mH$. Also recall some useful notations including $\mU=\frac{1}{\sqrt{d}}\1_d^\T$ and $\mV\triangleq \mW\otimes\mU$.

\begin{lemma}
\label{lemma:X-structure}
$\lambda_1(\trmX)=\frac{1}{2\pi}+\frac{\pi - 1}{2\pi d}$ with eigenvector $\frac{1}{\sqrt{d}}\1_d$. $\lambda_2(\trmX)=\dots=\lambda_d(\trmX)=\frac{\pi - 1}{2\pi d}.$
\end{lemma}

\begin{proofof}{\lemmaref{lemma:X-structure}}
From \equationref{eqn:xxT-structure} we know that \begin{equation}
    \trmX=\frac1d\ex{\rvx\rvx^\T}=\frac{1}{2\pi d}\1_d\1_d^\T+\frac{\pi - 1}{2\pi d}\mI_d.
\end{equation}
For unit vector $\vv=\frac{1}{\sqrt{d}}\1_d$, it satisfies
\begin{equation}
\begin{split}
    \trmX\vv = \frac{1}{2\pi d}\1_d\1_d^\T\frac{1}{\sqrt{d}}\1_d +\frac{\pi - 1}{2\pi d}\mI_d \frac{1}{\sqrt{d}}\1_d = \rbr{\frac{1}{2\pi}+\frac{\pi - 1}{2\pi d}} \frac{1}{\sqrt{d}}\1_d.
\end{split}
\end{equation}
Hence the all one vector has eigenvalue $\frac{1}{2\pi}+\frac{\pi - 1}{2\pi d}$.
For any unit vector $\vv\perp \1_d$, it satisfies
\begin{equation}
\begin{split}
    \trmX\vv = \frac{1}{2\pi d}\1_d\1_d^\T \vv +\frac{\pi - 1}{2\pi d}\mI_d\vv = \frac{\pi - 1}{2\pi d}\vv.
\end{split}
\end{equation}
Which means $\lambda_2=\lambda_3=\dots=\lambda_d=\frac{\pi - 1}{2\pi d}$.
\end{proofof}

\begin{corollary}
\label{cor:H-hat-eigenspace}
With probability 1 over $\mW^{(1)}$ and $\mW^{(2)}$, the overlap between the top $c-1$ eigenspace of $\hat\mH$ and $\gR\{\mV_i\}_{i=1}^c\backslash\{\mV\cdot\emph{\textbf{1}}\}$ converges to 1 as $n\to\infty$.
\end{corollary}
\begin{proofof}{\corollaryref{cor:H-hat-eigenspace}}
First note that by simple linear algebra,
\begin{equation}
\gR\{\mV_i\}_{i=1}^c\backslash\{\textbf{1}^\T\mV\}=(\gR\{\mW_i\}_{i=1}^c\backslash\{\mW\cdot\1\})\otimes \mU.
\end{equation}
While from \theoremref{thm:main-out} we know the overlap between the top $c-1$ eigenspace of $\mM$ and $\gR\{\mW_i\}_{i=1}^c\backslash\{\textbf{1}^\T\mW\}$ converges to 1. Thus for proving this corollary it is sufficient to show that the top $c-1$ eigenspace of $\frac1d\hat\mH = \mM\otimes \trmX$ is the Kronecker product of the top $c-1$ eigenspace of $\mM$ and $\mU$.

From \theoremref{thm:main-out} we know, with probability 1 over $\mW^{(1)}$ and $\mW^{(2)}$, for large $n$, $\lambda_{c-1}(\mM)>\eta/4$ and $\lambda_1(\mM)<2c^2$ where $\eta$ and $c$ are absolute constants. Thus for large $n$ we have \begin{equation}
\begin{split}
\lim_{n\to\infty}\lambda_1(\trmX)\lambda_{c-1}(\mM) &= \lim_{d\to\infty}\rbr{\frac{1}{2\pi}+\frac{\pi-1}{2\pi d}}\lambda_{c-1}(\mM)\geq \frac{1}{2\pi}\frac{\eta}{4}.
\end{split}
\end{equation}
while
\begin{equation}
\begin{split}
\lim_{n\to\infty}\lambda_2(\trmX)\lambda_1(\mM) &= \lim_{d\to\infty}\frac{\pi-1}{2\pi d}\lambda_{c-1}(\mM)\leq \lim_{d\to\infty}\frac{\pi-1}{2\pi d}2c^2=0.
\end{split}
\end{equation}
Since for large $n$, $\lambda_1(\trmX)\lambda_{c-1}(\mM) > \lambda_2(\trmX)\lambda_1(\mM)$, the top $c-1$ eigenspace of $\frac1d\hat\mH$ is the top $c-1$ eigenspace of $\mM$ Kronecker with the first eigenvector of $\trmX$, which is exactly $\mU$ from \lemmaref{lemma:X-structure}. This completes the proof of this corollary.

\end{proofof}

Now we proceed to prove the main theorem

\begin{proofof}{\theoremref{thm:main-full}}
We will conduct the proof on $\tmH=\frac{1}{d}\mH$ as the properties to be proved are invariant to scalar multiplication. From \corollaryref{cor:H-hat-eigenspace} we know the overlap between the top $c-1$ eigenspace of $\hat\mH$ and $\gR\{\mV_i\}_{i=1}^c\backslash\{\textbf{1}^\T\mV\}$ converges to 1. Thus we only need to show the overlap between the top $c-1$ eigenspace of $\tmH$ and $\gR\{\mV_i\}_{i=1}^c\backslash\{\textbf{1}^\T\mV\}$ converges to 1.

The proof strategy for the full layerwise Hessian is exactly the same as the proof for the output Hessian in \sectionref{sec:proof-A-structure}. In particular, the proof is nearly identical when we change the projection matrix from $P_\mW$ to $P_\mV$ where $\mV\triangleq \mW\otimes\mU$.

Therefore, instead of rewriting the entire proof, we may neglect some repeating arguments by verifying the equivalent lemmas for the full layer-wise Hessian.
With $\mV$ as defined, we have $\fn{\mV} = \fn{\mW}$, $\mV\mV^\T = \mW\mW^\T$, and $\fn{\mV^\T\mV} = \fn{\mW^\T\mW}$, so we can directly apply the exact same result of the two norm bounds (\lemmaref{lemma:W-norm}, \lemmaref{cor:WW-Identity}) on $\mV$. Now we prove \lemmaref{lemma:V-projection} as the equivalent of \lemmaref{lemma:W-projection}.


\begin{lemma}
\label{lemma:V-projection}
Let $\bmV\triangleq \bmW\otimes \mU$, then $P_\mV\triangleq \bmV^\T\bmV$ is the projection matrix from $\R^{nd}$ onto the subspace spanned by all rows of $\mV=\mW\otimes \mU$. Moreover, for all $\eps>0$, \begin{equation}
    \lim_{n\to\infty}\pr{\fns{\mV^\T\mV-P_\mV}>\eps} = 0.
\end{equation}
\end{lemma}

\begin{proofof}{\lemmaref{lemma:V-projection}}
Since Kronecker product with the constant $1\times d$ matrix $\mU$ preserves the orthogonality of vectors, doing Gram-Schmit on $\mV$ is equivalent to doing Gram-Schmit on $\mW$ then Kronecker with $\mU$, which results in $\bmV$ by construction. Therefore $P_\mV$ is a valid projection matrix.

Also note that for any $\mW$, \begin{equation}
\begin{split}
\fns{\mV^\T\mV-P_\mV}&=\fns{(\mW\otimes\mU)^\T(\mW\otimes\mU)-\bmV^\T\bmV}\\
&=\fns{(\mW^\T\mW)\otimes(\mU^\T\mU)-(\bmW^\T\bmW)\otimes(\mU^\T\mU)}\\
&=\fns{\mW^\T\mW-\bmW^\T\bmW}\fns{\mU^\T\mU}\\
&=\fns{\mW^\T\mW-\bmW^\T\bmW}\fns{\frac1d\1_d\1_d^\T}\\
&=\fns{\mW^\T\mW-P_\mW}.
\end{split}
\end{equation}
From \lemmaref{lemma:W-projection} we have
\begin{equation}
    \lim_{n\to\infty}\pr{\fns{\mV^\T\mV-P_\mV}>\eps} = \lim_{n\to\infty}\pr{\fns{\mW^\T\mW-P_\mW}>\eps}= 0.
\end{equation}
\end{proofof}

Note that the equivalent lemmas of \lemmaref{lemma:M-proj-preserve-f-norm}- \lemmaref{lemma:F-norm-equal} for $\tmH$ are also established in \lemmaref{lemma:H-proj-preserve-f-norm} - \lemmaref{lemma:F-norm-equal-H} in \sectionref{sec:proof-project}, substituting $(P_\mW, \mM, \mM^*)$ by $(P_\mV, \tmH, \tmH^*)$, we may follow the argument in \sectionref{sec:proof-out-hessian} up to \equationref{eqn:M-equal-WTWMWTW} and conclude that
\begin{equation}
\label{eqn:H-equal-VTVHVTV}
    \lim_{n\to\infty}\fn{\tmH-\mV^\T\mV\tmH^*\mV^\T\mV} = 0.
\end{equation}
Now claim an equivalent argument of \equationref{eqn:WTWMWTW-equal-WTAW}, that
\begin{equation}
\label{eqn:VTVHVTV-equal-VTAV}
    \lim_{n\to\infty}\fn{\frac{1}{8\pi}\mV^\T\tilde{\rmA}\mV - \mV^\T\mV\tmH^*\mV^\T\mV} = 0.
\end{equation}
Observe that 
\begin{equation}
\begin{split}
\mV^\T\trmA\mV
=(\mW\otimes\mU)^\T\trmA(\mW\otimes\mU) =  \mW^\T\trmA\mW\otimes\mU^\T\mU
\end{split}
\end{equation}
and
\begin{equation}
\begin{split}
\mV^\T\mV\tmH^*\mV^\T\mV &= (\mW\otimes\mU)^\T(\mW\otimes\mU)(\mM^*\otimes\trmX)(\mW\otimes\mU)^\T(\mW\otimes\mU)\\
&=\mW^\T\mW\mM^*\mW^\T\mW\otimes\mU^\T\mU\trmX\mU^\T\mU.
\end{split}
\end{equation}
We have\begin{equation}
\label{eqn:proof-VTVHVTV-equal-VTAV}
\begin{split}
    & \fn{\frac{1}{8\pi}\mV^\T\tilde{\rmA}\mV - \mV^\T\mV\tmH^*\mV^\T\mV}\\
    =\ &\fn{\frac{1}{8\pi}\mW^\T\trmA\mW\otimes\mU^\T\mU - \mW^\T\mW\mM^*\mW^\T\mW\otimes\mU^\T\mU\trmX\mU^\T\mU}\\
    \leq\ &\fn{\frac{1}{8\pi}\mW^\T\trmA\mW\otimes\mU^\T\mU - \frac{1}{2\pi}\mW^\T\mW\mM^*\mW^\T\mW\otimes\mU^\T\mU}\\
    &\ +\fn{\frac{1}{2\pi}\mW^\T\mW\mM^*\mW^\T\mW\otimes\mU^\T\mU - \mW^\T\mW\mM^*\mW^\T\mW\otimes\mU^\T\mU\trmX\mU^\T\mU}\\
    =\ &\frac{1}{2\pi}\fn{\frac14\mW^\T\trmA\mW-\mW^\T\mW\mM^*\mW^\T\mW}\fn{\mU^\T\mU\trmX\mU^\T\mU}\\
    &\ +\fn{\mW^\T\mW\mM^*\mW^\T\mW}\fn{\frac{1}{2\pi}\mU^\T\mU - \mU^\T\mU\trmX\mU^\T\mU}.
\end{split}
\end{equation}
Let's first consider the second term. Note that from \lemmaref{lemma:X-structure}, \begin{equation}
\begin{split}
    \fn{\frac{1}{2\pi}\mU^\T\mU - \mU^\T\mU\trmX\mU^\T\mU} &= \lfn{\frac{1}{2\pi d}\1_d\1_d^\T - \frac{1}{d^2}\rbr{\sum_{i,j=1}^d\frac{1}{d}\ex{\rvx\rvx^\T}_{ij}}\1_d\1_d^\T}\\
    &= \labs{\frac{1}{2\pi d} - \frac{1}{d^3}\rbr{\frac{2\pi d^2}{2\pi}+\frac{(\pi-1)d}{2\pi}}}\lfn{\1_d\1_d^\T}\\
    &= \frac{\pi-1}{2\pi d^2}d = \frac{\pi-1}{2\pi d}.
\end{split}
\end{equation}
Which converges to $0$ as $n\to\infty$ (since $d = n^{1+\alpha}$).
Since $\fn{\mW^\T\mW\mM^*\mW^\T\mW}$ is bounded above from \lemmaref{lemma:W-norm} and \lemmaref{lemma:M-star}. We have 
\begin{equation}
\label{eqn:VTVHVTV-equal-VTAV-sub1}
    \lim_{n\to\infty} \fn{\mW^\T\mW\mM^*\mW^\T\mW}\fn{\frac{1}{2\pi}\mU^\T\mU - \mU^\T\mU\trmX\mU^\T\mU} = 0.
\end{equation}
For the first term, since for all $d$,
\begin{equation}
\begin{split}
\fn{\mU^\T\mU\trmX\mU^\T\mU} &= \lfn{\frac{1}{d^2}\rbr{\sum_{i,j=1}^d\frac{1}{d}\ex{\rvx\rvx^\T}_{ij}}\1_d\1_d^\T}\\
&= \frac{1}{d^2}\rbr{\frac{2\pi d^2}{2\pi}+\frac{(\pi-1)d}{2\pi}} < \frac{1}{2},
\end{split}
\end{equation}
Combined with \equationref{eqn:WTWMWTW-equal-WTAW} we have\begin{equation}
\label{eqn:VTVHVTV-equal-VTAV-sub2}
    \lim_{n\to\infty}\frac{1}{2\pi}\fn{\frac14\mW^\T\trmA\mW-\mW^\T\mW\mM^*\mW^\T\mW}\fn{\mU^\T\mU\trmX\mU^\T\mU} = 0.
\end{equation}
Plug \equationref{eqn:VTVHVTV-equal-VTAV-sub1} and \equationref{eqn:VTVHVTV-equal-VTAV-sub2} into \equationref{eqn:proof-VTVHVTV-equal-VTAV} gives us \equationref{eqn:VTVHVTV-equal-VTAV}.

Now substitute $\frac{1}{4}\mW^\T\mA\mW$ in \sectionref{sec:proof-out-hessian} to $\frac{1}{8\pi}\mV^\T\mA\mV$, following the arguments after \equationref{eqn:WTWMWTW-equal-WTAW} completes the remaining proof for this theorem.
\end{proofof}